Packlore

DeBruijnSSA/BinSyntax/Rewrite/Term/Compose/Structural.lean
@@ -1,6 +1,7 @@
 import DeBruijnSSA.BinSyntax.Rewrite.Term.Compose.Seq
 import DeBruijnSSA.BinSyntax.Rewrite.Term.Compose.Sum
-import DeBruijnSSA.BinSyntax.Typing.Region.Structural
+import DeBruijnSSA.BinSyntax.Rewrite.Term.Compose.Product
+import DeBruijnSSA.BinSyntax.Typing.Term.Structural
 
 
 namespace BinSyntax
@@ -27,20 +28,83 @@ theorem Eqv.pack_sum_def {Γ : Ctx α ε} {R : LCtx α} {i : Fin R.length}
       ext
       simp [Term.pack0, Term.Wf.pack0, -Function.iterate_succ, Function.iterate_succ']
 
-def Eqv.pack {Γ : Ctx α ε} : Eqv φ Γ (Γ.pack, Γ.sup_effect) := match Γ with
+def Eqv.pack' {Γ : Ctx α ε} : Eqv φ Γ (Γ.pack, Γ.sup_effect) := match Γ with
   | [] => unit ⊥
-  | V::Γ => pair (var 0 (by cases V; simp)) ((pack (Γ := Γ)).wk0.wk_eff (by simp))
+  | V::Γ => pair (var 0 (by cases V; simp)) ((pack' (Γ := Γ)).wk0.wk_eff (by simp))
 
-def _root_.BinSyntax.Ctx.Pure.packE {Γ : Ctx α ε} (h : Γ.Pure) : Eqv φ Γ (Γ.pack, ⊥) := match Γ with
+theorem Eqv.pack_def' {Γ : Ctx α ε} : Eqv.pack' (φ := φ) (Γ := Γ) = ⟦Term.InS.pack'⟧ := by
+  induction Γ with
+  | nil => rfl
+  | cons _ _ I => simp only [pack', I]; rfl
+
+def _root_.BinSyntax.Ctx.Pure.packE' {Γ : Ctx α ε} (h : Γ.Pure) : Eqv φ Γ (Γ.pack, ⊥) := match Γ with
   | [] => Eqv.unit ⊥
-  | V::Γ => Eqv.pair (Eqv.var 0 (by cases V; convert h.head; simp)) h.tail.packE.wk0
+  | V::Γ => Eqv.pair (Eqv.var 0 (by cases V; convert h.head; simp)) h.tail.packE'.wk0
 
-def Eqv.unpack {Γ Δ : Ctx α ε} (i : Fin Γ.length) : Eqv φ ((Γ.pack, ⊥)::Δ) ((Γ.get i).1, e)
+theorem Eqv.packE_def' {Γ : Ctx α ε} {h : Γ.Pure} : h.packE' (φ := φ) = ⟦h.pack'⟧ := by
+  induction Γ with
+  | nil => rfl
+  | cons _ _ I => simp only [Ctx.Pure.packE', I]; rfl
+
+def Eqv.pack_drop {Γ Δ : Ctx α ε} (i : Fin Γ.length)
+  : Eqv φ ((Γ.pack, ⊥)::Δ) (Ctx.pack (Γ.drop i), e)
+  := ⟦InS.pack_drop i⟧
+
+def Eqv.pack_drop' {Γ Δ : Ctx α ε} (i : Fin Γ.length)
+  : Eqv φ ((Γ.pack, ⊥)::Δ) ((Γ.get i).1.prod (Ctx.pack (Γ.drop (i + 1))), e)
+  := ⟦InS.pack_drop' i⟧
+
+theorem Eqv.cast_pack_drop {Γ Δ : Ctx α ε} {i : Fin Γ.length}
+  : (Eqv.pack_drop (φ := φ) (Δ := Δ) (e := e) i).cast rfl (by rw [Ctx.pack_drop_fin]) = pack_drop' i
+  := rfl
+
+theorem Eqv.cast_pack_drop' {Γ Δ : Ctx α ε} {i : Fin Γ.length}
+  : (Eqv.pack_drop' (φ := φ) (Δ := Δ) (e := e) i).cast rfl (by rw [<-Ctx.pack_drop_fin])
+  = pack_drop i
+  := rfl
+
+def Eqv.pack_drop_succ {Γ Δ : Ctx α ε} (i : Fin Γ.length)
+  : pack_drop (φ := φ)  (Γ := V::Γ) (Δ := Δ) (e := e) i.succ
+  = (pack_drop' (φ := φ) (Γ := V::Γ) (Δ := Δ) (e := e) i.castSucc).pr := by
+  simp only [pack_drop, InS.pack_drop_succ]; rfl
+
+def Eqv.unpack0 {Γ Δ : Ctx α ε} (i : Fin Γ.length) : Eqv φ ((Γ.pack, ⊥)::Δ) ((Γ.get i).1, e)
+  := ⟦InS.unpack0 i⟧
+
+theorem Eqv.pl_pack_drop'  {Γ Δ : Ctx α ε} {i : Fin Γ.length}
+  : (Eqv.pack_drop' (φ := φ) (Δ := Δ) (e := e) i).pl = unpack0 i := rfl
+
+theorem Eqv.unpack0_def {Γ Δ : Ctx α ε} (i : Fin Γ.length) :
+  Eqv.unpack0 (φ := φ) (Δ := Δ) (e := e) i = ⟦Term.InS.unpack0 i⟧ := rfl
+
+def Eqv.unpack0' {Γ Δ : Ctx α ε} (i : Fin Γ.length) : Eqv φ ((Γ.pack, ⊥)::Δ) ((Γ.get i).1, e)
   := match Γ with
   | [] => i.elim0
   | V::Γ => let2
     (var (V := (V.1.prod (Ctx.pack Γ), e)) 0 (by simp [Ctx.pack]))
-    (i.cases (var 1 (by simp)) (λi => unpack i))
+    (i.cases (var 1 (by simp)) (λi => unpack0' i))
+
+theorem Eqv.unpack0_def' {Γ Δ : Ctx α ε} (i : Fin Γ.length) :
+  unpack0' (φ := φ) (Δ := Δ) (e := e) i = ⟦Term.InS.unpack0' i⟧ := by
+  induction Γ generalizing Δ with
+  | nil => exact i.elim0
+  | cons _ _ I =>
+    simp only [
+      List.get_eq_getElem, List.length_cons, unpack0', var, Fin.val_zero,
+      List.getElem_cons_zero, I, InS.unpack0'
+    ]
+    cases i using Fin.cases <;> rfl
+
+-- theorem Eqv.unpack0_eq_unpack0' {Γ Δ : Ctx α ε} (i : Fin Γ.length) :
+--   Eqv.unpack0 (φ := φ) (Δ := Δ) (e := e) i = Eqv.unpack0' i := by
+--   cases Γ with
+--   | nil => exact i.elim0
+--   | cons V Γ =>
+--   induction i using Fin.induction generalizing Δ with
+--   | zero => rfl
+--   | succ =>
+--     simp [unpack0', <-pl_pack_drop', <-cast_pack_drop, pack_drop_succ]
+--     sorry
 
 -- TODO: wk lift unpack
 
