DeBruijnSSA/BinSyntax/Typing/Region/Structural.lean
@@ -1,77 +1,10 @@
-import DeBruijnSSA.BinSyntax.Typing.Ctx
-import DeBruijnSSA.BinSyntax.Typing.LCtx
-import DeBruijnSSA.BinSyntax.Typing.Term.Basic
+import DeBruijnSSA.BinSyntax.Typing.Term.Structural
 import DeBruijnSSA.BinSyntax.Typing.Region.LSubst
 import DeBruijnSSA.BinSyntax.Typing.Region.Compose
 
 namespace BinSyntax
 
 namespace Term
-
-variable
-  [Φ: EffInstSet φ (Ty α) ε] [PartialOrder α] [PartialOrder ε] [OrderBot ε]
-  {Γ Δ : Ctx α ε} {σ : Region.Subst φ}
-
-def pack0 (ℓ : ℕ) : Term φ := inr^[ℓ] (inl (var 0))
-
-@[simp]
-theorem wk_lift_pack0 {ℓ : ℕ} : (pack0 ℓ).wk (Nat.liftWk ρ) = pack0 (φ := φ) ℓ := by
-  simp only [pack0]
-  induction ℓ with
-  | zero => rfl
-  | succ ℓ ih => simp [ih, -Function.iterate_succ, Function.iterate_succ']
-
-@[simp]
-theorem wk1_pack0 : (pack0 ℓ).wk1 = pack0 (φ := φ) ℓ := by
-  simp only [wk1, wk_lift_pack0]
-
-@[simp]
-theorem subst_lift_pack0 {ℓ : ℕ} {σ : Subst φ} : (pack0 ℓ).subst σ.lift = pack0 (φ := φ) ℓ := by
-  simp only [pack0]
-  induction ℓ with
-  | zero => rfl
-  | succ ℓ ih => simp [ih, -Function.iterate_succ, Function.iterate_succ']
-
-@[simp]
-theorem Wf.pack0 {Γ : Ctx α ε} {R : LCtx α} {i : Fin R.length}
-  : Term.Wf (φ := φ) ((R.get i, ⊥)::Γ) (pack0 i) (R.pack, ⊥)  := by
-  induction R generalizing Γ with
-  | nil => exact i.elim0
-  | cons _ _ I =>
-    cases i using Fin.cases with
-    | zero => exact Wf.inl $ Wf.var Ctx.Var.shead
-    | succ i =>
-      simp only [Fin.val_succ,
-        BinSyntax.Term.pack0, Function.iterate_succ', Function.comp_apply, LCtx.pack, Wf.inr_iff]
-      apply I
-
-def InS.pack0 {Γ : Ctx α ε} (R : LCtx α) (i : Fin R.length)
-  : Term.InS φ ((R.get i, ⊥)::Γ) (R.pack, ⊥) :=
-  ⟨Term.pack0 i, Term.Wf.pack0⟩
-
-@[simp]
-theorem InS.coe_pack {Γ : Ctx α ε} {R : LCtx α} {i : Fin R.length}
-  : (InS.pack0 (φ := φ) (Γ := Γ) (R := R) i : Term φ) = Term.pack0 i := rfl
-
-@[simp]
-theorem InS.wk_lift_pack0 {Γ : Ctx α ε} {R : LCtx α} {i : Fin R.length} {ρ : Γ.InS Δ}
-  : (InS.pack0 (φ := φ) R i).wk (ρ.lift (le_refl _)) = pack0 R i := by ext; simp
-
-@[simp]
-theorem InS.wk_slift_pack0 {Γ : Ctx α ε} {R : LCtx α} {i : Fin R.length} {ρ : Γ.InS Δ}
-  : (InS.pack0 (φ := φ) R i).wk (ρ.slift) = pack0 R i := by ext; simp
-
-@[simp]
-theorem InS.subst_lift_pack0 {Γ : Ctx α ε} {R : LCtx α} {i : Fin R.length} {σ : Subst.InS φ Γ Δ}
-  : (InS.pack0 (φ := φ) R i).subst (σ.lift (le_refl _)) = pack0 R i := by ext; simp
-
-@[simp]
-theorem InS.subst_slift_pack0 {Γ : Ctx α ε} {R : LCtx α} {i : Fin R.length} {σ : Subst.InS φ Γ Δ}
-  : (InS.pack0 (φ := φ) R i).subst σ.slift = pack0 R i := by ext; simp
-
-@[simp]
-theorem InS.wk1_pack0 {Γ : Ctx α ε} {R : LCtx α} {i : Fin R.length}
-  : (InS.pack0 (φ := φ) (Γ := Γ) R i).wk1 (inserted := inserted) = pack0 R i := by ext; simp
 
 end Term
 
