DeBruijnSSA/BinSyntax/Typing/Term/Structural.lean
@@ -1,0 +1,220 @@
+import DeBruijnSSA.BinSyntax.Typing.Term.Subst
+import DeBruijnSSA.BinSyntax.Typing.Term.Compose
+import DeBruijnSSA.BinSyntax.Typing.LCtx
+
+namespace BinSyntax
+
+namespace Term
+
+section Product
+
+variable
+  [Φ: EffInstSet φ (Ty α) ε] [PartialOrder α] [SemilatticeSup ε] [OrderBot ε]
+  {Γ Δ : Ctx α ε} {σ : Region.Subst φ}
+
+def pack : ℕ → Term φ
+  | 0 => unit
+  | n + 1 => pair (var 0) (pack n).wk0
+
+theorem Wf.pack {Γ Δ : Ctx α ε}
+  : Wf (φ := φ) (Γ ++ Δ) (pack Γ.length) (Γ.pack, Γ.sup_effect) := by
+  induction Γ with
+  | nil => exact Wf.unit _
+  | cons V Γ I =>
+    simp only [List.cons_append, BinSyntax.Term.pack, Ctx.pack, Ctx.sup_effect, pair_iff, var_iff,
+      Ctx.Var.head_iff, ge_iff_le]
+    constructor
+    constructor
+    rfl
+    simp
+    apply Wf.wk0
+    apply Wf.wk_eff _ I
+    simp
+
+theorem Wf.pack' {Γ : Ctx α ε}
+  : Wf (φ := φ) Γ (Term.pack Γ.length) (Γ.pack, Γ.sup_effect) :=
+  by convert Wf.pack (Δ := []); simp
+
+def InS.pack' {Γ : Ctx α ε} : InS φ Γ (Γ.pack, Γ.sup_effect) := match Γ with
+  | [] => unit ⊥
+  | V::Γ => pair (var 0 (by cases V; simp)) ((pack' (Γ := Γ)).wk0.wk_eff (by simp))
+
+@[simp]
+theorem InS.coe_pack' {Γ : Ctx α ε} : (InS.pack' (φ := φ) (Γ := Γ) : Term φ) = Term.pack Γ.length
+  := by induction Γ with
+  | nil => rfl
+  | cons => simp [pack', Term.pack, *]
+
+def _root_.BinSyntax.Ctx.Pure.pack' {Γ : Ctx α ε} (h : Γ.Pure) : InS φ Γ (Γ.pack, ⊥) := match Γ with
+  | [] => InS.unit ⊥
+  | V::Γ => InS.pair (InS.var 0 (by cases V; convert h.head; simp)) h.tail.pack'.wk0
+
+@[simp]
+theorem InS.coe_pure_pack {Γ : Ctx α ε} {h : Γ.Pure}
+  : (h.pack' (φ := φ) : Term φ) = Term.pack Γ.length := by induction Γ with
+  | nil => rfl
+  | cons => simp [Term.pack, Ctx.Pure.pack', *]
+
+theorem InS.wk_eff_coe_pure' {Γ : Ctx α ε} {h : Γ.Pure}
+  : (h.pack' (φ := φ)).wk_eff bot_le = pack' := by ext; simp
+
+def unpack0 (x : ℕ) : Term φ := pl (pr^[x] (var 0))
+
+theorem Wf.pack_drop' {Γ Δ : Ctx α ε} {i : ℕ} (hi : i < Γ.length)
+  : Wf (φ := φ) ((Γ.pack, ⊥)::Δ) (Term.pr^[i] (Term.var 0))
+      ((Γ.get ⟨i, hi⟩).1.prod (Ctx.pack (Γ.drop (i + 1))), e)
+  := by induction i generalizing Γ with
+  | zero => cases Γ with
+    | nil => cases hi
+    | cons _ Γ => simp [unpack0, Ctx.pack]
+  | succ i I => cases Γ with
+    | nil => cases hi
+    | cons head Γ =>
+      simp only [BinSyntax.Term.unpack0, List.length_cons, Fin.val_succ, Function.iterate_succ',
+        Function.comp_apply, List.get_eq_getElem, List.getElem_cons_succ, Ctx.pack]
+      apply Wf.pr
+      convert I (Γ := head::Γ) (Nat.lt_of_succ_lt hi)
+      simp only [List.drop_succ_cons]
+      simp only [List.length_cons, add_lt_add_iff_right] at hi
+      clear I
+      induction Γ generalizing i with
+      | nil => cases hi
+      | cons head Γ I =>
+        cases i with
+        | zero => rfl
+        | succ i =>
+          simp only [List.getElem_cons_succ, List.drop_succ_cons]
+          apply I
+          exact hi
+          simp only [List.length_cons, add_lt_add_iff_right] at hi
+          exact hi
+
+theorem Wf.pack_drop {Γ Δ : Ctx α ε} {i : ℕ} (hi : i < Γ.length)
+  : Wf (φ := φ) ((Γ.pack, ⊥)::Δ) (Term.pr^[i] (Term.var 0)) (Ctx.pack (Γ.drop i), e)
+  := by rw [Ctx.pack_drop hi]; apply Wf.pack_drop' hi
+
+theorem Wf.unpack0 {Γ Δ : Ctx α ε} {i : Fin Γ.length}
+  : Wf (φ := φ) ((Γ.pack, ⊥)::Δ) (unpack0 i) ((Γ.get i).1, e)
+  := Wf.pl (pack_drop' i.prop)
+
+def InS.pack_drop {Γ Δ : Ctx α ε} (i : Fin Γ.length)
+  : InS φ ((Γ.pack, ⊥)::Δ) (Ctx.pack (Γ.drop i), e)
+  := ⟨Term.pr^[i] (Term.var 0), Wf.pack_drop i.prop⟩
+
+@[simp]
+theorem InS.coe_pack_drop {Γ Δ : Ctx α ε} {i : Fin Γ.length}
+  : (InS.pack_drop (φ := φ) (Δ := Δ) (e := e) i : Term φ) = Term.pr^[i] (Term.var 0) := rfl
+
+def InS.pack_drop' {Γ Δ : Ctx α ε} (i : Fin Γ.length)
+  : InS φ ((Γ.pack, ⊥)::Δ) ((Γ.get i).1.prod (Ctx.pack (Γ.drop (i + 1))), e)
+  := ⟨Term.pr^[i] (Term.var 0), Wf.pack_drop' i.prop⟩
+
+@[simp]
+theorem InS.coe_pack_drop' {Γ Δ : Ctx α ε} {i : Fin Γ.length}
+  : (InS.pack_drop' (φ := φ) (Δ := Δ) (e := e) i : Term φ) = Term.pr^[i] (Term.var 0) := rfl
+
+theorem InS.cast_pack_drop {Γ Δ : Ctx α ε} {i : Fin Γ.length}
+  : (InS.pack_drop (φ := φ) (Δ := Δ) (e := e) i).cast rfl (by rw [Ctx.pack_drop_fin]) = pack_drop' i
+  := rfl
+
+theorem InS.cast_pack_drop' {Γ Δ : Ctx α ε} {i : Fin Γ.length}
+  : (InS.pack_drop' (φ := φ) (Δ := Δ) (e := e) i).cast rfl (by rw [<-Ctx.pack_drop_fin])
+  = pack_drop i
+  := rfl
+
+def InS.pack_drop_succ {Γ Δ : Ctx α ε} (i : Fin Γ.length)
+  : pack_drop (φ := φ)  (Γ := V::Γ) (Δ := Δ) (e := e) i.succ
+  = (pack_drop' (φ := φ) (Γ := V::Γ) (Δ := Δ) (e := e) i.castSucc).pr := by
+  ext; simp only [List.length_cons, Fin.val_succ, List.drop_succ_cons, Set.mem_setOf_eq,
+    coe_pack_drop, Function.iterate_succ, Function.comp_apply, Term.pr, List.get_eq_getElem,
+    Fin.coe_castSucc, coe_pr, coe_pack_drop']
+  rw [<-Term.pr, <-Function.iterate_succ_apply, Function.iterate_succ_apply']
+  rfl
+
+def InS.unpack0 {Γ Δ : Ctx α ε} (i : Fin Γ.length)
+  : InS φ ((Γ.pack, ⊥)::Δ) ((Γ.get i).1, e)
+  := ⟨Term.unpack0 i, Wf.unpack0⟩
+
+theorem InS.pl_pack_drop' {Γ Δ : Ctx α ε} {i : Fin Γ.length}
+  : (InS.pack_drop' (φ := φ) (Δ := Δ) (e := e) i).pl = unpack0 i := rfl
+
+theorem InS.coe_unpack0 {Γ Δ : Ctx α ε} {i : Fin Γ.length}
+  : (InS.unpack0 (φ := φ) (Δ := Δ) (e := e) i : Term φ) = Term.unpack0 i := rfl
+
+def InS.unpack0' {Γ Δ : Ctx α ε} (i : Fin Γ.length) : InS φ ((Γ.pack, ⊥)::Δ) ((Γ.get i).1, e)
+  := match Γ with
+  | [] => i.elim0
+  | V::Γ => let2
+    (var (V := (V.1.prod (Ctx.pack Γ), e)) 0 (by simp [Ctx.pack]))
+    (i.cases (var 1 (by simp)) (λi => unpack0' i))
+
+end Product
+
+section Sum
+
+variable
+  [Φ: EffInstSet φ (Ty α) ε] [PartialOrder α] [PartialOrder ε] [OrderBot ε]
+  {Γ Δ : Ctx α ε} {σ : Region.Subst φ}
+
+def pack0 (ℓ : ℕ) : Term φ := inr^[ℓ] (inl (var 0))
+
+@[simp]
+theorem wk_lift_pack0 {ℓ : ℕ} : (pack0 ℓ).wk (Nat.liftWk ρ) = pack0 (φ := φ) ℓ := by
+  simp only [pack0]
+  induction ℓ with
+  | zero => rfl
+  | succ ℓ ih => simp [ih, -Function.iterate_succ, Function.iterate_succ']
+
+@[simp]
+theorem wk1_pack0 : (pack0 ℓ).wk1 = pack0 (φ := φ) ℓ := by
+  simp only [wk1, wk_lift_pack0]
+
+@[simp]
+theorem subst_lift_pack0 {ℓ : ℕ} {σ : Subst φ} : (pack0 ℓ).subst σ.lift = pack0 (φ := φ) ℓ := by
+  simp only [pack0]
+  induction ℓ with
+  | zero => rfl
+  | succ ℓ ih => simp [ih, -Function.iterate_succ, Function.iterate_succ']
+
+@[simp]
+theorem Wf.pack0 {Γ : Ctx α ε} {R : LCtx α} {i : Fin R.length}
+  : Term.Wf (φ := φ) ((R.get i, ⊥)::Γ) (pack0 i) (R.pack, ⊥)  := by
+  induction R generalizing Γ with
+  | nil => exact i.elim0
+  | cons _ _ I =>
+    cases i using Fin.cases with
+    | zero => exact Wf.inl $ Wf.var Ctx.Var.shead
+    | succ i =>
+      simp only [Fin.val_succ,
+        BinSyntax.Term.pack0, Function.iterate_succ', Function.comp_apply, LCtx.pack, Wf.inr_iff]
+      apply I
+
+def InS.pack0 {Γ : Ctx α ε} (R : LCtx α) (i : Fin R.length)
+  : Term.InS φ ((R.get i, ⊥)::Γ) (R.pack, ⊥) :=
+  ⟨Term.pack0 i, Term.Wf.pack0⟩
+
+@[simp]
+theorem InS.coe_pack0 {Γ : Ctx α ε} {R : LCtx α} {i : Fin R.length}
+  : (InS.pack0 (φ := φ) (Γ := Γ) (R := R) i : Term φ) = Term.pack0 i := rfl
+
+@[simp]
+theorem InS.wk_lift_pack0 {Γ : Ctx α ε} {R : LCtx α} {i : Fin R.length} {ρ : Γ.InS Δ}
+  : (InS.pack0 (φ := φ) R i).wk (ρ.lift (le_refl _)) = pack0 R i := by ext; simp
+
+@[simp]
+theorem InS.wk_slift_pack0 {Γ : Ctx α ε} {R : LCtx α} {i : Fin R.length} {ρ : Γ.InS Δ}
+  : (InS.pack0 (φ := φ) R i).wk (ρ.slift) = pack0 R i := by ext; simp
+
+@[simp]
+theorem InS.subst_lift_pack0 {Γ : Ctx α ε} {R : LCtx α} {i : Fin R.length} {σ : Subst.InS φ Γ Δ}
+  : (InS.pack0 (φ := φ) R i).subst (σ.lift (le_refl _)) = pack0 R i := by ext; simp
+
+@[simp]
+theorem InS.subst_slift_pack0 {Γ : Ctx α ε} {R : LCtx α} {i : Fin R.length} {σ : Subst.InS φ Γ Δ}
+  : (InS.pack0 (φ := φ) R i).subst σ.slift = pack0 R i := by ext; simp
+
+@[simp]
+theorem InS.wk1_pack0 {Γ : Ctx α ε} {R : LCtx α} {i : Fin R.length}
+  : (InS.pack0 (φ := φ) (Γ := Γ) R i).wk1 (inserted := inserted) = pack0 R i := by ext; simp
+
+end Sum
